%%%%%%%%%%%%%%%%%%%%%%%%%%%%%%%%%%%%%%%%%%%%%%%%%%%%%%%%%%%%%%%%%%%%%%%%%%%%%%%%
\section{Mathematical Expressions\label{app:a}}
%%%%%%%%%%%%%%%%%%%%%%%%%%%%%%%%%%%%%%%%%%%%%%%%%%%%%%%%%%%%%%%%%%%%%%%%%%%%%%%%

%%%%%%%%%%%%%%%%%%%%%%%%%%%%%%%%%%%%%%%%%%%%%%%%%%%%%%%%%%%%%%%%%%%%%%%%%%%%%%%%

\subsection{Rotation transformations\label{appendix:rotational_transformations}}
%%%%%%%%%%%%%%%%%%%%%%%%%%%%%%%%%%%%%%%%%%%%%%%%%%%%%%%%%%%%%%%%%%%%%%%%%%%%%%%%

\begin{equation}
    \mathbb{T}_x(\phi_x)=
    \begin{bmatrix}
        1 & 0           & 0          \\
        0 & \cos\phi_x  & \sin\phi_x \\
        0 & -\sin\phi_x & \cos\phi_x \\
    \end{bmatrix}
\end{equation}

\begin{equation}
    \mathbb{T}_y(\phi_y)=
    \begin{bmatrix}
        \cos\phi_y  & 0 & -\sin\phi_y \\
        0           & 1 & 0           \\
        -\sin\phi_y & 0 & \cos\phi_y  \\
    \end{bmatrix}
\end{equation}

\begin{equation}
    \mathbb{T}_z(\phi_z)=
    \begin{bmatrix}
        \cos\phi_z  & \sin\phi_z & 0 \\
        -\sin\phi_z & \cos\phi_z & 0 \\
        0           & 0          & 1 \\
    \end{bmatrix}
\end{equation}

%%%%%%%%%%%%%%%%%%%%%%%%%%%%%%%%%%%%%%%%%%%%%%%%%%%%%%%%%%%%%%%%%%%%%%%%%%%%%%%%

\subsection{Incomplete integrals\label{appendix:incomplete_integrals}}
%%%%%%%%%%%%%%%%%%%%%%%%%%%%%%%%%%%%%%%%%%%%%%%%%%%%%%%%%%%%%%%%%%%%%%%%%%%%%%%%

\begin{equation}
    U(r_x, r_y, r_z) = G\int_V\frac{\rho{(s_x,s_y,s_z)}}{\sqrt{(r_x-s_x)^2+(r_y-s_y)^2+(r_z-s_z)^2}}\;dx\;dy\;dz
    \label{eq:ur-gen-rect}
\end{equation}

\begin{equation}
    R_F\!\left(x, y, z\right) = \frac{1}{2} \int_{0}^{\infty} \frac{1}{\sqrt{t + x} \sqrt{t + y} \sqrt{t + z}} \, dt
    \label{eq:elliptic_RF}
\end{equation}

\begin{equation}
    R_D\!\left(x, y, z\right) = \frac{3}{2} \int_{0}^{\infty} \frac{1}{\left(t + x\right) \left(t + y\right) {\left(t + z\right)}^{3 / 2}} \, dt
    \label{eq:elliptic_RD}
\end{equation}


%%%%%%%%%%%%%%%%%%%%%%%%%%%%%%%%%%%%%%%%%%%%%%%%%%%%%%%%%%%%%%%%%%%%%%%%%%%%%%%%

\subsection{Vector norms\label{appendix:vector_norms}}
%%%%%%%%%%%%%%%%%%%%%%%%%%%%%%%%%%%%%%%%%%%%%%%%%%%%%%%%%%%%%%%%%%%%%%%%%%%%%%%%
Given $x\in\gls{set:R}^n$, the vector norms for $\ell_p(\mathbf{x})$ are defined
by the following equations:

\begin{equation}
    \ell_1(\mathbf{x})=||\mathbf{x}||_1 = \sum_{d=1}^n |x_d|
\end{equation}

\begin{equation}
    \ell_2(\mathbf{x})=||\mathbf{x}||_2 = \sqrt{\sum_{d=1}^n x_d^2}
\end{equation}

\begin{equation}
    \ell_\infty(\mathbf{x})=||\mathbf{x}||_\infty = \max_{1\leq{d}\leq{n}}^n |x_d|
\end{equation}

\begin{equation}
    \ell_p(\mathbf{x})=||\mathbf{x}||_p=
    \begin{cases}
        \bigg(\sum_{d=1}^n |x_d|^p\bigg)^{1/p}    &  1\leq{}p\le \infty \\
        \max_{1\leq{d}\leq{n}}^n |x_d|            &  p=\infty \\
    \end{cases}
    \label{eq:ell-p}
\end{equation}

